Add arithmetic spec lemmas

backends/lean/Base/Primitives/Scalar.lean
@@ -3,6 +3,8 @@ import Lean.Meta.Tactic.Simp
 import Mathlib.Tactic.Linarith
 import Base.Primitives.Base
 import Base.Diverge.Base
+import Base.Progress.Base
+import Base.Arith.Int
 
 namespace Primitives
 
@@ -121,6 +123,22 @@ inductive ScalarTy :=
 | U32
 | U64
 | U128
+
+def ScalarTy.isSigned (ty : ScalarTy) : Bool :=
+  match ty with
+  | Isize
+  | I8
+  | I16
+  | I32
+  | I64
+  | I128 => true
+  | Usize
+  | U8
+  | U16
+  | U32
+  | U64
+  | U128 => false
+
 
 def Scalar.smin (ty : ScalarTy) : Int :=
   match ty with
@@ -289,22 +307,29 @@ def Scalar.tryMk (ty : ScalarTy) (x : Int) : Result (Scalar ty) :=
 
 def Scalar.neg {ty : ScalarTy} (x : Scalar ty) : Result (Scalar ty) := Scalar.tryMk ty (- x.val)
 
-def Scalar.div {ty : ScalarTy} (x : Scalar ty) (y : Scalar ty) : Result (Scalar ty) :=
-  if y.val != 0 then Scalar.tryMk ty (x.val / y.val) else fail divisionByZero
-
 -- Our custom remainder operation, which satisfies the semantics of Rust
 -- TODO: is there a better way?
 def scalar_rem (x y : Int) : Int :=
-  if 0 ≤ x then |x| % |y|
+  if 0 ≤ x then x % y
   else - (|x| % |y|)
+
+@[simp]
+def scalar_rem_nonneg {x y : Int} (hx : 0 ≤ x) : scalar_rem x y = x % y := by
+  intros
+  simp [*, scalar_rem]
 
 -- Our custom division operation, which satisfies the semantics of Rust
 -- TODO: is there a better way?
 def scalar_div (x y : Int) : Int :=
-  if 0 ≤ x && 0 ≤ y then |x| / |y|
+  if 0 ≤ x && 0 ≤ y then x / y
   else if 0 ≤ x && y < 0 then - (|x| / |y|)
   else if x < 0 && 0 ≤ y then - (|x| / |y|)
   else |x| / |y|
+
+@[simp]
+def scalar_div_nonneg {x y : Int} (hx : 0 ≤ x) (hy : 0 ≤ y) : scalar_div x y = x / y := by
+  intros
+  simp [*, scalar_div]
 
 -- Checking that the remainder operation is correct
 #assert scalar_rem 1 2 = 1
@@ -326,8 +351,11 @@ def scalar_div (x y : Int) : Int :=
 #assert scalar_div 7 (-3) = -2
 #assert scalar_div (-7) (-3) = 2
 
+def Scalar.div {ty : ScalarTy} (x : Scalar ty) (y : Scalar ty) : Result (Scalar ty) :=
+  if y.val != 0 then Scalar.tryMk ty (scalar_div x.val y.val) else fail divisionByZero
+
 def Scalar.rem {ty : ScalarTy} (x : Scalar ty) (y : Scalar ty) : Result (Scalar ty) :=
-  if y.val != 0 then Scalar.tryMk ty (x.val % y.val) else fail divisionByZero
+  if y.val != 0 then Scalar.tryMk ty (scalar_rem x.val y.val) else fail divisionByZero
 
 def Scalar.add {ty : ScalarTy} (x : Scalar ty) (y : Scalar ty) : Result (Scalar ty) :=
   Scalar.tryMk ty (x.val + y.val)
@@ -409,6 +437,133 @@ instance {ty} : HDiv (Scalar ty) (Scalar ty) (Result (Scalar ty)) where
 -- Remainder
 instance {ty} : HMod (Scalar ty) (Scalar ty) (Result (Scalar ty)) where
   hMod x y := Scalar.rem x y
+
+-- TODO: make progress work at a more fine grained level (see `Scalar.add_unsigned_spec`)
+@[cpspec]
+theorem Scalar.add_spec {ty} {x y : Scalar ty}
+  (hmin : Scalar.min ty ≤ x.val + y.val)
+  (hmax : x.val + y.val ≤ Scalar.max ty) :
+  ∃ z, x + y = ret z ∧ z.val = x.val + y.val := by
+  simp [HAdd.hAdd, add, Add.add]
+  simp [tryMk]
+  split
+  . simp [pure]
+    rfl
+  . tauto
+
+theorem Scalar.add_unsigned_spec {ty} (s: ¬ ty.isSigned) {x y : Scalar ty}
+  (hmax : x.val + y.val ≤ Scalar.max ty) :
+  ∃ z, x + y = ret z ∧ z.val = x.val + y.val := by
+  have hmin : Scalar.min ty ≤ x.val + y.val := by
+    have hx := x.hmin
+    have hy := y.hmin
+    cases ty <;> simp [min] at * <;> linarith
+  apply add_spec <;> assumption
+
+-- TODO: make it finer grained
+@[cpspec]
+theorem Scalar.sub_spec {ty} {x y : Scalar ty}
+  (hmin : Scalar.min ty ≤ x.val - y.val)
+  (hmax : x.val - y.val ≤ Scalar.max ty) :
+  ∃ z, x - y = ret z ∧ z.val = x.val - y.val := by
+  simp [HSub.hSub, sub, Sub.sub]
+  simp [tryMk]
+  split
+  . simp [pure]
+    rfl
+  . tauto
+
+theorem Scalar.sub_unsigned_spec {ty} (s: ¬ ty.isSigned) {x y : Scalar ty}
+  (hmin : Scalar.min ty ≤ x.val - y.val) :
+  ∃ z, x - y = ret z ∧ z.val = x.val - y.val := by
+  have : x.val - y.val ≤ Scalar.max ty := by
+    have hx := x.hmin
+    have hxm := x.hmax
+    have hy := y.hmin
+    cases ty <;> simp [min, max] at * <;> linarith
+  intros
+  apply sub_spec <;> assumption
+
+-- TODO: make it finer grained
+@[cpspec]
+theorem Scalar.mul_spec {ty} {x y : Scalar ty}
+  (hmin : Scalar.min ty ≤ x.val * y.val)
+  (hmax : x.val * y.val ≤ Scalar.max ty) :
+  ∃ z, x * y = ret z ∧ z.val = x.val * y.val := by
+  simp [HMul.hMul, mul, Mul.mul]
+  simp [tryMk]
+  split
+  . simp [pure]
+    rfl
+  . tauto
+
+theorem Scalar.mul_unsigned_spec {ty} (s: ¬ ty.isSigned) {x y : Scalar ty}
+  (hmax : x.val * y.val ≤ Scalar.max ty) :
+  ∃ z, x * y = ret z ∧ z.val = x.val * y.val := by
+  have : Scalar.min ty ≤ x.val * y.val := by
+    have hx := x.hmin
+    have hy := y.hmin
+    cases ty <;> simp at * <;> apply mul_nonneg hx hy
+  apply mul_spec <;> assumption
+
+-- TODO: make it finer grained
+@[cpspec]
+theorem Scalar.div_spec {ty} {x y : Scalar ty}
+  (hnz : y.val ≠ 0)
+  (hmin : Scalar.min ty ≤ scalar_div x.val y.val)
+  (hmax : scalar_div x.val y.val ≤ Scalar.max ty) :
+  ∃ z, x / y = ret z ∧ z.val = scalar_div x.val y.val := by
+  simp [HDiv.hDiv, div, Div.div]
+  simp [tryMk, *]
+  simp [pure]
+  rfl
+
+theorem Scalar.div_unsigned_spec {ty} (s: ¬ ty.isSigned) (x : Scalar ty) {y : Scalar ty}
+  (hnz : y.val ≠ 0) :
+  ∃ z, x / y = ret z ∧ z.val = x.val / y.val := by
+  have h : Scalar.min ty = 0 := by cases ty <;> simp at *
+  have hx := x.hmin
+  have hy := y.hmin
+  simp [h] at hx hy
+  have hmin : 0 ≤ x.val / y.val := Int.ediv_nonneg hx hy
+  have hmax : x.val / y.val ≤ Scalar.max ty := by
+    have := Int.ediv_le_self y.val hx
+    have := x.hmax
+    linarith
+  have hs := @div_spec ty x y hnz
+  simp [*] at hs
+  apply hs
+
+-- TODO: make it finer grained
+@[cpspec]
+theorem Scalar.rem_spec {ty} {x y : Scalar ty}
+  (hnz : y.val ≠ 0)
+  (hmin : Scalar.min ty ≤ scalar_rem x.val y.val)
+  (hmax : scalar_rem x.val y.val ≤ Scalar.max ty) :
+  ∃ z, x % y = ret z ∧ z.val = scalar_rem x.val y.val := by
+  simp [HMod.hMod, rem]
+  simp [tryMk, *]
+  simp [pure]
+  rfl
+
+theorem Scalar.rem_unsigned_spec {ty} (s: ¬ ty.isSigned) (x : Scalar ty) {y : Scalar ty}
+  (hnz : y.val ≠ 0) :
+  ∃ z, x % y = ret z ∧ z.val = scalar_rem x.val y.val := by
+  have h : Scalar.min ty = 0 := by cases ty <;> simp at *
+  have hx := x.hmin
+  have hy := y.hmin
+  simp [h] at hx hy
+  have hmin : 0 ≤ x.val % y.val := Int.emod_nonneg x.val hnz
+  have hmax : x.val % y.val ≤ Scalar.max ty := by
+    have h := @Int.ediv_emod_unique x.val y.val (x.val % y.val) (x.val / y.val)
+    simp at h
+    have : 0 < y.val := by int_tac
+    simp [*] at h
+    have := y.hmax
+    linarith
+  have hs := @rem_spec ty x y hnz
+  simp [*] at hs
+  simp [*]
 
 -- ofIntCore
 -- TODO: typeclass?
